[constraints][3/X] add generics constraints
Adding a set of constraints to all subtyping judgements, and fallout.
No new rules are added, and one admit had to be added into adequacy.

The next diff will add the new subtyping rules to use these constraints
and the necessary checks (New / Class and Method defs), but won't fix
adequacy. The diff after that will tie the knot and fix everything.

theories/typing.v
@@ -14,9 +14,9 @@ Section Typing.
   Context `{PDC: ProgDefContext}.
 
   (* Helping the inference with this notation that hides Δ *)
-  Local Notation "s <: t" := (@subtype _ s t) (at level 70, no associativity).
-  Local Notation "lty <:< rty" := (@lty_sub _ lty rty) (at level 70, no associativity).
-  Local Notation "lts <: vs :> rts" := (@subtype_targs _ vs lts rts) (at level 70, vs at next level).
+  Local Notation "Γ ⊢ s <: t" := (@subtype _ Γ s t) (at level 70, s at next level, no associativity).
+  Local Notation "Γ ⊢ lts <: vs :> rts" := (@subtype_targs _ Γ vs lts rts) (at level 70, lts, vs at next level).
+  Local Notation "Γ ⊢ lty <:< rty" := (@lty_sub _ Γ lty rty) (lty at next level, at level 70, no associativity).
 
   (* Typing Judgements *)
   Definition is_bool_op op : bool :=
@@ -26,37 +26,37 @@ Section Typing.
     end
   .
 
-  Inductive expr_has_ty (lty : local_tys) :
+  Inductive expr_has_ty Γ (lty : local_tys) :
     expr → lang_ty → Prop :=
-    | IntTy : ∀ z, expr_has_ty lty (IntE z) IntT
-    | BoolTy: ∀ b, expr_has_ty lty (BoolE b) BoolT
-    | NullTy: expr_has_ty lty NullE NullT
+    | IntTy : ∀ z, expr_has_ty Γ lty (IntE z) IntT
+    | BoolTy: ∀ b, expr_has_ty Γ lty (BoolE b) BoolT
+    | NullTy: expr_has_ty Γ lty NullE NullT
     | OpIntTy: ∀ op e1 e2,
         is_bool_op op = false →
-        expr_has_ty lty e1 IntT →
-        expr_has_ty lty e2 IntT →
-        expr_has_ty lty (OpE op e1 e2) IntT
+        expr_has_ty Γ lty e1 IntT →
+        expr_has_ty Γ lty e2 IntT →
+        expr_has_ty Γ lty (OpE op e1 e2) IntT
     | OpBoolTy: ∀ op e1 e2,
         is_bool_op op = true →
-        expr_has_ty lty e1 IntT →
-        expr_has_ty lty e2 IntT →
-        expr_has_ty lty (OpE op e1 e2) BoolT
+        expr_has_ty Γ lty e1 IntT →
+        expr_has_ty Γ lty e2 IntT →
+        expr_has_ty Γ lty (OpE op e1 e2) BoolT
     | GenTy: ∀ v ty,
         lty.(ctxt) !! v = Some ty →
-        expr_has_ty lty (VarE v) ty
-    | ThisTy : expr_has_ty lty ThisE (this_type lty)
+        expr_has_ty Γ lty (VarE v) ty
+    | ThisTy : expr_has_ty Γ lty ThisE (this_type lty)
     | ESubTy: ∀ e s t,
-        expr_has_ty lty e s →
+        expr_has_ty Γ lty e s →
         wf_ty t →
-        s <: t →
-        expr_has_ty lty e t
+        Γ ⊢ s <: t →
+        expr_has_ty Γ lty e t
   .
 
-  Lemma expr_has_ty_subst σ lty e ty:
+  Lemma expr_has_ty_subst Γ σ lty e ty:
     map_Forall (λ _ : string, wf_cdef_parent Δ) Δ →
     Forall wf_ty σ →
-    expr_has_ty lty e ty →
-    expr_has_ty (subst_lty σ lty) e (subst_ty σ ty).
+    expr_has_ty Γ lty e ty →
+    expr_has_ty (subst_constraints σ Γ) (subst_lty σ lty) e (subst_ty σ ty).
   Proof.
     move => hp hwf.
     induction 1 as [ z | b | | op e1 e2 hop h1 hi1 h2 hi2 |
@@ -105,9 +105,9 @@ Section Typing.
       by apply hl in hk.
   Qed.
 
-  Lemma expr_has_ty_wf lty e ty:
+  Lemma expr_has_ty_wf Γ lty e ty:
     wf_lty lty →
-    expr_has_ty lty e ty →
+    expr_has_ty Γ lty e ty →
     wf_ty ty.
   Proof.
     move => hwf.
@@ -118,39 +118,38 @@ Section Typing.
   Qed.
 
   (* continuation-based typing for commands *)
-  Inductive cmd_has_ty :
-    local_tys → cmd → local_tys → Prop :=
-    | SkipTy: ∀ lty, cmd_has_ty lty SkipC lty
+  Inductive cmd_has_ty Γ : local_tys → cmd → local_tys → Prop :=
+    | SkipTy: ∀ lty, cmd_has_ty Γ lty SkipC lty
     | SeqTy: ∀ lty1 lty2 lty3 fstc sndc,
-        cmd_has_ty lty1 fstc lty2 →
-        cmd_has_ty lty2 sndc lty3 →
-        cmd_has_ty lty1 (SeqC fstc sndc) lty3
+        cmd_has_ty Γ lty1 fstc lty2 →
+        cmd_has_ty Γ lty2 sndc lty3 →
+        cmd_has_ty Γ lty1 (SeqC fstc sndc) lty3
     | LetTy: ∀ lty lhs e ty,
-        expr_has_ty lty e ty →
-        cmd_has_ty lty (LetC lhs e) (<[lhs := ty]>lty)
+        expr_has_ty Γ lty e ty →
+        cmd_has_ty Γ lty (LetC lhs e) (<[lhs := ty]>lty)
     | IfTy: ∀ lty1 lty2 cond thn els,
-        expr_has_ty lty1 cond BoolT →
-        cmd_has_ty lty1 thn lty2 →
-        cmd_has_ty lty1 els lty2 →
-        cmd_has_ty lty1 (IfC cond thn els) lty2
+        expr_has_ty Γ lty1 cond BoolT →
+        cmd_has_ty Γ lty1 thn lty2 →
+        cmd_has_ty Γ lty1 els lty2 →
+        cmd_has_ty Γ lty1 (IfC cond thn els) lty2
     | GetPrivTy: ∀ lty lhs t σ name fty,
         type_of_this lty = (t, σ) →
         has_field name t Private fty t →
-        cmd_has_ty lty (GetC lhs ThisE name) (<[lhs := subst_ty σ fty]>lty)
+        cmd_has_ty Γ lty (GetC lhs ThisE name) (<[lhs := subst_ty σ fty]>lty)
     | GetPubTy: ∀ lty lhs recv t σ name fty orig,
-        expr_has_ty lty recv (ClassT t σ) →
+        expr_has_ty Γ lty recv (ClassT t σ) →
         has_field name t Public fty orig →
-        cmd_has_ty lty (GetC lhs recv name) (<[lhs := subst_ty σ fty]>lty)
+        cmd_has_ty Γ lty (GetC lhs recv name) (<[lhs := subst_ty σ fty]>lty)
     | SetPrivTy: ∀ lty fld rhs fty t σ,
         type_of_this lty = (t, σ) →
         has_field fld t Private fty t →
-        expr_has_ty lty rhs (subst_ty σ fty) →
-        cmd_has_ty lty (SetC ThisE fld rhs) lty
+        expr_has_ty Γ lty rhs (subst_ty σ fty) →
+        cmd_has_ty Γ lty (SetC ThisE fld rhs) lty
     | SetPubTy: ∀ lty recv fld rhs fty orig t σ,
-        expr_has_ty lty recv (ClassT t σ) →
+        expr_has_ty Γ lty recv (ClassT t σ) →
         has_field fld t Public fty orig →
-        expr_has_ty lty rhs (subst_ty σ fty) →
-        cmd_has_ty lty (SetC recv fld rhs) lty
+        expr_has_ty Γ lty rhs (subst_ty σ fty) →
+        cmd_has_ty Γ lty (SetC recv fld rhs) lty
     | NewTy: ∀ lty lhs t targs args fields (*cdef*),
         wf_ty (ClassT t targs) →
         has_fields t fields →
@@ -158,34 +157,34 @@ Section Typing.
         (∀ f fty arg,
         fields !! f = Some fty →
         args !! f = Some arg →
-        expr_has_ty lty arg (subst_ty targs fty.1.2)) →
-        cmd_has_ty lty (NewC lhs t args) (<[lhs := ClassT t targs]>lty)
+        expr_has_ty Γ lty arg (subst_ty targs fty.1.2)) →
+        cmd_has_ty Γ lty (NewC lhs t args) (<[lhs := ClassT t targs]>lty)
     | CallTy: ∀ lty lhs recv t targs name orig mdef args,
-        expr_has_ty lty recv (ClassT t targs) →
+        expr_has_ty Γ lty recv (ClassT t targs) →
         has_method name t orig mdef →
         dom (gset string) mdef.(methodargs) = dom _ args →
         (∀ x ty arg,
         mdef.(methodargs) !! x = Some ty →
         args !! x = Some arg →
-        expr_has_ty lty arg (subst_ty targs ty)) →
-        cmd_has_ty lty (CallC lhs recv name args) (<[lhs := subst_ty targs mdef.(methodrettype)]>lty)
+        expr_has_ty Γ lty arg (subst_ty targs ty)) →
+        cmd_has_ty Γ lty (CallC lhs recv name args) (<[lhs := subst_ty targs mdef.(methodrettype)]>lty)
     | SubTy: ∀ lty c rty rty',
-        rty' <:< rty →
-        cmd_has_ty lty c rty' →
-        cmd_has_ty lty c rty
+        Γ ⊢ rty' <:< rty →
+        cmd_has_ty Γ lty c rty' →
+        cmd_has_ty Γ lty c rty
     | CondTagTy lty rty v tv t cmd :
         lty.(ctxt) !! v = Some tv →
-        lty <:< rty →
-        cmd_has_ty (<[v:=InterT tv (ExT t)]> lty) cmd rty →
-        cmd_has_ty lty (CondTagC v t cmd) rty
+        Γ ⊢ lty <:< rty →
+        cmd_has_ty Γ (<[v:=InterT tv (ExT t)]> lty) cmd rty →
+        cmd_has_ty Γ lty (CondTagC v t cmd) rty
   .
 
-  Lemma cmd_has_ty_wf lty cmd lty' :
+  Lemma cmd_has_ty_wf Γ lty cmd lty' :
     map_Forall (λ _ : string, wf_cdef_parent Δ) Δ →
     map_Forall (λ _ : string, wf_cdef_fields_wf) Δ →
     map_Forall (λ _ : string, wf_cdef_methods_wf) Δ →
     wf_lty lty →
-    cmd_has_ty lty cmd lty' →
+    cmd_has_ty Γ lty cmd lty' →
     wf_lty lty'.
   Proof.
     move => hp hfields hmethods [hthis hwf].
@@ -243,7 +242,7 @@ Section Typing.
         by apply hwf in hk.
   Qed.
 
-  Lemma cmd_has_ty_subst σ lty cmd lty':
+  Lemma cmd_has_ty_subst Γ σ lty cmd lty':
     map_Forall (λ _ : string, wf_cdef_parent Δ) Δ →
     map_Forall (λ _ : string, wf_cdef_fields_wf) Δ →
     map_Forall (λ _ : string, wf_cdef_methods_wf) Δ →
@@ -251,8 +250,8 @@ Section Typing.
     map_Forall (λ _ : string, cdef_methods_bounded) Δ →
     wf_lty lty →
     Forall wf_ty σ →
-    cmd_has_ty lty cmd lty' →
-    cmd_has_ty (subst_lty σ lty) cmd (subst_lty σ lty').
+    cmd_has_ty Γ lty cmd lty' →
+    cmd_has_ty (subst_constraints σ Γ) (subst_lty σ lty) cmd (subst_lty σ lty').
   Proof.
     move => hp hfields hmethods hfb hmb hwf0 hwf1.
     induction 1 as [ lty | ????? h1 hi1 h2 hi2 | ???? he |
@@ -396,18 +395,18 @@ Section Typing.
    * method bodies must be well-formed under a generic substitution mapping
    * Ti -> Ti.
    *)
-  Definition wf_mdef_ty tag σ σ' mdef :=
+  Definition wf_mdef_ty Γ tag σ σ' mdef :=
     ∃ rty,
     wf_lty rty ∧
-    cmd_has_ty
+    cmd_has_ty Γ
       {| type_of_this := (tag, σ); ctxt := subst_ty σ' <$> mdef.(methodargs) |}
       mdef.(methodbody) rty ∧
-    expr_has_ty rty mdef.(methodret) (subst_ty σ' mdef.(methodrettype))
+    expr_has_ty Γ rty mdef.(methodret) (subst_ty σ' mdef.(methodrettype))
   .
 
   Definition cdef_wf_mdef_ty cname cdef :=
     let σ := gen_targs (length cdef.(generics)) in
-    map_Forall (λ _mname mdef, wf_mdef_ty cname σ σ mdef) cdef.(classmethods)
+    map_Forall (λ _mname mdef, wf_mdef_ty cdef.(constraints) cname σ σ mdef) cdef.(classmethods)
   .
 
   (* Collection of all program invariant (at the source level):
